\def\newex#1{\noindent{\bf #1} }
\def\ldot{\,.\,}
\def\alphaeq{=_\alpha}
\def\betatr{\to_\beta}
\newex{1.1} (a) $$\eqalign{
(\lambda x\ldot(((xz)y)(xx)))
&\equiv\lambda x\ldot(((xz)y)(xx))\cr
&\equiv\lambda x\ldot((xz)y)(xx)\cr
&\equiv\lambda x\ldot(xz)y(xx)\cr
&\equiv\lambda x\ldot xzy(xx)\cr}$$
(b) $$\eqalign{
((\lambda x\ldot(\lambda y\ldot(\lambda z\ldot(z((xy)z)))))(\lambda u\ldot u))
&\equiv(\lambda x\ldot(\lambda y\ldot(\lambda z\ldot(z((xy)z)))))(\lambda u\ldot u)\cr
&\equiv(\lambda xy\ldot(\lambda z\ldot(z((xy)z))))(\lambda u\ldot u)\cr
&\equiv(\lambda xyz\ldot(z((xy)z)))(\lambda u\ldot u)\cr
&\equiv(\lambda xyz\ldot z((xy)z))(\lambda u\ldot u)\cr
&\equiv(\lambda xyz\ldot z(xyz))(\lambda u\ldot u)\cr}$$

\newex{1.2} (a) Yes. (b) No, $y\in FV(y)$ but $x$ is a binding variable.
(c) No, $x\in FV(x)$.

\newex{1.3} Given $z\notin FV(x(\lambda z\ldot y))$ and $x\notin FV(\lambda z\ldot y)$, $$
\eqalign{\lambda x\ldot x(\lambda z\ldot y)
&\alphaeq \lambda z \ldot (x(\lambda z\ldot y))^{x\to z}\cr
&\equiv \lambda z \ldot z(\lambda z\ldot y).\cr}$$

\newex{1.4} (a) $$
\{(\lambda z\ldot zxz)((\lambda y\ldot xy)x),
(\lambda z\ldot zxz), ((\lambda y\ldot xy)x),
zxz, (\lambda y\ldot xy), x,
zx, xy,
y, z
\}.$$
(b) (TODO)\par\noindent
(c) $$
\eqalign{
FV(U)
&= FV(\lambda z\ldot zxz)\cup FV((\lambda y\ldot xy)x)\cr
&= (FV(zxz)\!\setminus\!\{z\})\cup(FV(\lambda y\ldot xy)\cup FV(x))\cr
&= \{x\} \cup \{x\}\cr
&= \{x\}\cr
}
$$
(d) Given the lemma, $$
M_1N_1\alphaeq M_2N_2 \iff M_1\alphaeq M_2 \quad\hbox{and}\quad N_1\alphaeq N_2,
$$ it's easy to reduce the original problems to smaller problems.

\newex{1.5} (a) $$
\eqalign{
(\lambda x\ldot y(\lambda y\ldot xy))[y := \lambda z\ldot zx]
&\equiv\lambda u\ldot (y(\lambda y\ldot uy))[y := \lambda z\ldot zx]\cr
&\equiv\lambda u\ldot y[y := \lambda z\ldot zx](\lambda y\ldot uy)[y := \lambda z\ldot zx]\cr
&\equiv\lambda u\ldot (\lambda z\ldot zx)(\lambda v\ldot uv)[y := \lambda z\ldot zx]\cr
&\equiv\lambda u\ldot (\lambda z\ldot zx)(\lambda v\ldot (uv)[y := \lambda z\ldot zx])\cr
&\equiv\lambda u\ldot (\lambda z\ldot zx)(\lambda v\ldot uv)\cr
}
$$
(b) $$
\eqalign{
((xyz)[x:=y])[y:=z]
&\equiv((xy)[x:=y]z)[y:=z]\cr
&\equiv(x[x:=y]yz)[y:=z]\cr
&\equiv(yyz)[y:=z]\cr
&\equiv zzz\cr
}
$$
(c) $$
\eqalign{
((\lambda x\ldot xyz)[x:=y])[y:=z]
&\equiv(\lambda u\ldot (uyz)[x:=y])[y:=z]\cr
&\equiv(\lambda u\ldot (uyz))[y:=z]\cr
&\equiv\lambda u\ldot (uyz)[y:=z]\cr
&\equiv\lambda u\ldot uzz\cr
}
$$
(d) $$
\eqalign{
(\lambda y\ldot yyx)[x:=yz]
&\equiv\lambda u\ldot (uux)[x:=yz]\cr
&\equiv\lambda u\ldot uu(yz)\cr
}
$$

\newex{1.6} Try $M:=xy$, $N:=y$, $L:=z$, then $$
(xy)[x:=y, y:=z]\equiv yz,
$$
but $$
(xy)[x:=y][y:=z]\equiv zz.
$$

\newex{1.7} (a) $(\lambda z\ldot zxz)((\lambda y\ldot xy)x)$ and $(\lambda y\ldot xy)x$.\par\noindent
(b) First, $$
\eqalign{(\lambda z\ldot zxz)((\lambda y\ldot xy)x)
&\betatr ((\lambda y\ldot xy)x)x((\lambda y\ldot xy)x)\cr
&\betatr xxx((\lambda y\ldot xy)x)\cr
&\betatr xxx(xx),\cr}$$
Second, $$
\eqalign{(\lambda z\ldot zxz)((\lambda y\ldot xy)x)
&\betatr ((\lambda y\ldot xy)x)x((\lambda y\ldot xy)x)\cr
&\betatr ((\lambda y\ldot xy)x)x(xx)\cr
&\betatr xxx(xx),\cr}$$
Third, $$
\eqalign{(\lambda z\ldot zxz)((\lambda y\ldot xy)x)
&\betatr (\lambda z\ldot zxz)(xx)\cr
&\betatr xxx(xx),\cr}$$

\bye
